\documentclass[10pt]{article}
\usepackage[usenames]{color} %used for font color
\usepackage[top=1.0in,bottom=1.0in,left=1.0in,right=1.0in]{geometry}

\input{math_commands_for_appendices.tex}

\title{Connections between (Entropy Regularized) Policy Gradient and Mirror Descent with Neural Networks}
\author{}
\date{}

\begin{document}

\maketitle

\begin{lem}
Let $\rvr_1, \rvr_2, \dots, \rvr_t \in \left[ 0, 1  \right]^K$. Denote $\rvr_{1:t} \triangleq \sum\limits_{i=1}^{t}{\rvr_i}$, and $\hat{\rvr}_t \triangleq \frac{\rvr_{1:t}}{t}$. Let $\rvo \in \sR^K$ be any logit vector, and $\rvpi(\rvo)$ be the softmax policy of $\rvo$. Denote $\rmH\left( \rvpi \left(\rvo \right) \right) \triangleq \Delta \left( \rvpi \left(\rvo \right) \right) - \rvpi \left(\rvo \right) \rvpi \left(\rvo \right)^\top$, where $\Delta \left( \rvpi \left(\rvo \right) \right) \in \sR^{K \times K}$ is a matrix with $\rvpi \left(\rvo \right)$ as its diagonal. Define the policy gradient with respect to logit at step $t$,
\begin{equation*}
\begin{split}
    \nabla(\rvo_t) &\triangleq \frac{d \left\{ \rvpi(\rvo_t)^\top \rvr_t - \rvpi(\rvo_t)^\top \log{\rvpi(\rvo_t)} \right\} }{d \rvo_t} \\
    &= \left[ \Delta \left( \rvpi(\rvo_t) \right) - \rvpi(\rvo_t) \rvpi(\rvo_t)^\top \right] \left( \rvr_t - \rvo_t \right) \\
    &\triangleq \rmH_t \left( \rvr_t - \rvo_t \right).
\end{split}
\end{equation*}
Consider the following (entropy regularized) policy gradient update,
\begin{equation*}
\begin{split}
    \rvo_{t+1} &= \rvo_t + \eta \cdot \nabla(\rvo_t) \\
    &= \rvo_t + \eta \cdot \rmH_t \left( \rvr_t - \rvo_t \right).
\end{split}
\end{equation*}
If the learning rate $\eta$ satisfies
\begin{equation*}
    \frac{1}{t+1} + \frac{1}{(t+1)(t+C)} \le \eta \cdot \lambda_{\min}\left\{ \rmH_t \right\} \le 1,
\end{equation*}
then we have,
\begin{equation*}
    \left\| \rvo_{t+1} - \hat{\rvr}_{t} - c \cdot \rvone \right\| \le \frac{C \cdot \sqrt{K}}{t+1}.
\end{equation*}
\end{lem}
\begin{proof}
According to the update,
\begin{equation*}
\begin{split}
    \rvo_{t+1} - \hat{\rvr}_t - c \cdot \rvone &= \rvo_{t} - \hat{\rvr}_{t-1} - c \cdot \rvone + \hat{\rvr}_{t-1} - \hat{\rvr}_t - \eta \cdot \rmH_t \left( \rvo_{t} - \hat{\rvr}_{t-1} - c \cdot \rvone \right) - \eta \cdot \rmH_t \left( \hat{\rvr}_{t-1} - \rvr_t \right),
\end{split}
\end{equation*}
where $c \in \sR$ is a constant. Denote $\rvdelta_{t} \triangleq \rvo_{t} - \hat{\rvr}_{t-1} - c \cdot \rvone$, and note,
\begin{equation*}
\begin{split}
    \hat{\rvr}_{t-1} - \hat{\rvr}_t &= \frac{\rvr_{1:t-1}}{t-1} - \frac{\rvr_{1:t-1} + \rvr_t}{t} = \frac{\rvr_{1:t-1} - (t-1) \cdot \rvr_t }{t(t-1)} = \frac{1}{t} \cdot \left( \hat{\rvr}_{t-1} - \rvr_t \right).
\end{split}
\end{equation*}
We have the following result,
\begin{equation*}
\begin{split}
    \rvdelta_{t+1} = \left[ \rmI - \eta \cdot \rmH_t \right] \rvdelta_t + \left[ \frac{1}{t} \cdot \rmI - \eta \cdot \rmH_t \right] \left( \hat{\rvr}_{t-1} - \rvr_t \right).
\end{split}
\end{equation*}
By the triangle and H{\" o}lder's inequality,
\begin{equation*}
\begin{split}
    \left\| \rvdelta_{t+1} \right\| &\le \lambda_{\max}\left\{ \rmI - \eta \cdot \rmH_t \right\} \cdot \left\| \rvdelta_{t} \right\| + \lambda_{\max}\left\{ \frac{1}{t} \cdot \rmI - \eta \cdot \rmH_t \right\} \cdot \left\| \hat{\rvr}_{t-1} - \rvr_t \right\| \\
    &\le \left( 1 - \eta \cdot \lambda_{\min}\left\{ \rmH_t \right\} \right) \cdot \left\| \rvdelta_{t} \right\| + \left( \frac{1}{t} - \eta \cdot \lambda_{\min}\left\{ \rmH_t \right\} \right) \cdot \sqrt{K}.
\end{split}
\end{equation*}
We use induction on $t$. For $t = 0$, $\rvdelta_{1} = \rvzero$, and $\left\| \rvdelta_{1} \right\| \le C \cdot \sqrt{K}$. Assume the result holds for $t$, then for $t+1$,
\begin{equation*}
\begin{split}
    \left\| \rvdelta_{t+1} \right\| &\le \left( 1 - \eta \cdot \lambda_{\min}\left\{ \rmH_t \right\} \right) \cdot \frac{C \cdot \sqrt{K}}{t} + \left( \frac{1}{t} - \eta \cdot \lambda_{\min}\left\{ \rmH_t \right\} \right) \cdot \sqrt{K} \\
    &= \frac{C \cdot \sqrt{K}}{t} + \frac{\sqrt{K}}{t} - \eta \cdot \lambda_{\min}\left\{ \rmH_t \right\} \cdot \left( \frac{C \cdot \sqrt{K}}{t} + \sqrt{K} \right) \\
    &\le \frac{C \cdot \sqrt{K}}{t} + \frac{\sqrt{K}}{t} - \left[ \frac{1}{t+1} + \frac{1}{(t+1)(t+C)} \right] \cdot \left( \frac{C \cdot \sqrt{K}}{t} + \sqrt{K} \right) \\
    &= \frac{C \cdot \sqrt{K}}{t+1}. \qedhere
\end{split}
\end{equation*}
\end{proof}

\begin{lem}
Given any $\rvpi \in \Delta$, define $\rmH\left( \rvpi \right) \triangleq \Delta \left( \rvpi \right) - \rvpi \rvpi^\top$. Sorting $\rvpi$ in ascending order,
\begin{equation*}
\begin{split}
    &\quad \rvpi(1) = \rvpi(2) = \cdots = \rvpi(|\gS_1|) \\
    &< \rvpi(|\gS_1|+1) = \rvpi(|\gS_1|+2) = \cdots = \rvpi(|\gS_1| + |\gS_2|) \\
    &\ \ \vdots \\
    &< \rvpi(K - |\gS_k| + 1) = \rvpi(K - |\gS_k| + 2) = \cdots = \rvpi(K),
\end{split}
\end{equation*}
where $\gS_i \triangleq \left\{ \rvpi(|\gS_{<i}| + 1), \rvpi(|\gS_{<i}| + 2), \dots,  \rvpi(|\gS_{<i}| + |\gS_i|) \right\}$, $\forall 1 \le i \le k$, and $|\gS_{<i}| \triangleq \sum\limits_{j < i}{|\gS_j|}$ satisfy \begin{equation*}
\begin{split}
    \bigcup_{i=1}^{k}{\gS_i} &= \left\{ \rvpi(1), \rvpi(2), \dots, \rvpi(K) \right\} \\
    \gS_i \cap \gS_j &= \emptyset, \quad \forall i \not= j.
\end{split}    
\end{equation*}
Then the eigenvalues of $\rmH\left( \rvpi \right)$ are
\begin{equation*}
\begin{split}
    \lambda_{1} &= 0 \\
    \lambda_{2} = \lambda_{3} = \cdots = \lambda_{|\gS_1|} &= \rvpi(|\gS_1|) \\
    \lambda_{|\gS_1| + 1 } &\in \left( \rvpi(|\gS_1|), \rvpi(|\gS_2|) \right) \\
    \lambda_{|\gS_1| + 2} = \lambda_{|\gS_1| + 3} = \cdots = \lambda_{|\gS_1| + |\gS_2|} &= \rvpi(|\gS_2|) \\
    \lambda_{|\gS_1| + |\gS_2| + 1 } &\in \left( \rvpi(|\gS_2|), \rvpi(|\gS_3|) \right) \\
    &\ \ \vdots \\
    \lambda_{K - |\gS_k| +1} &\in \left( \rvpi(K-1), \rvpi(K) \right) \\
    \lambda_{K - |\gS_k| + 2} = \lambda_{K - |\gS_k| + 3} = \cdots = \lambda_{K} &= \rvpi(K).
\end{split}
\end{equation*}
And for any eigenvalue $\lambda$ of $\rmH(\rvpi)$ such that $\lambda \not= \rvpi(i)$, $\forall i \in [K]$, we have
\begin{equation*}
    \sum\limits_{i=1}^{K}{\frac{\rvpi(i)^2}{\rvpi(i) - \lambda}} = 1.
\end{equation*}
\end{lem}
\begin{proof}
Suppose $\lambda$ is an eigenvalue of $\rmH(\rvpi)$ and $\rvv$ is the corresponding eigenvector, i.e.,
\begin{equation*}
    \rmH(\rvpi) \rvv = \left[ \Delta(\rvpi) - \rvpi\rvpi^\top \right] \rvv = \lambda \rvv.
\end{equation*}
It is easy to check that $\rvv = \rvone$ is the eigenvector of $\lambda_0 = 0$. Next, assuming $\lambda \not= 0$, we have
\begin{equation*}
    \rvpi(i) \left( \rvv(i) - \rvpi^\top \rvv \right) = \lambda \rvv(i), \quad \forall i \in [K].
\end{equation*}
Note if $\rvpi^\top \rvv = 0$, we have $\rvpi(i) \rvv(i) = \lambda \rvv(i)$, $\forall i \in [K]$. Since $\rvv \not= \rvzero$, assume 
\end{proof}

\end{document}